Renamed stack -> evaluation context

EvaluationContext.thy
@@ -1,4 +1,4 @@
-theory Stack
+theory EvaluationContext
 imports Typecheck Misc
 begin
 
@@ -10,13 +10,13 @@ inductive typecheck_frame :: "nat \<Rightarrow> type list \<Rightarrow> frame \<
 
 inductive_cases [elim]: "\<Delta>,\<Gamma> \<turnstile> f : t \<rightarrow> t'"
 
-inductive typecheck_stack :: "nat \<Rightarrow> type list \<Rightarrow> frame list \<Rightarrow> type \<Rightarrow> type \<Rightarrow> bool" 
-    (infix ",_ \<turnstile>\<^sub>s _ : _ \<rightarrow>" 60) where
-  tcs_nil [simp]: "\<Delta>,\<Gamma> \<turnstile>\<^sub>s [] : t \<rightarrow> t"
-| tcs_cons [simp]: "\<Delta>,\<Gamma> \<turnstile>\<^sub>s s : t\<^sub>1 \<rightarrow> t\<^sub>2 \<Longrightarrow> \<Delta>,\<Gamma> \<turnstile> f : t\<^sub>2 \<rightarrow> t\<^sub>3 \<Longrightarrow> \<Delta>,\<Gamma> \<turnstile>\<^sub>s f # s : t\<^sub>1 \<rightarrow> t\<^sub>3"
+inductive typecheck_context :: "nat \<Rightarrow> type list \<Rightarrow> frame list \<Rightarrow> type \<Rightarrow> type \<Rightarrow> bool" 
+    (infix ",_ \<turnstile>\<^sub>e\<^sub>c _ : _ \<rightarrow>" 60) where
+  tcec_nil [simp]: "\<Delta>,\<Gamma> \<turnstile>\<^sub>e\<^sub>c [] : t \<rightarrow> t"
+| tcec_cons [simp]: "\<Delta>,\<Gamma> \<turnstile>\<^sub>e\<^sub>c s : t\<^sub>1 \<rightarrow> t\<^sub>2 \<Longrightarrow> \<Delta>,\<Gamma> \<turnstile> f : t\<^sub>2 \<rightarrow> t\<^sub>3 \<Longrightarrow> \<Delta>,\<Gamma> \<turnstile>\<^sub>e\<^sub>c f # s : t\<^sub>1 \<rightarrow> t\<^sub>3"
 
-inductive_cases [elim]: "\<Delta>,\<Gamma> \<turnstile>\<^sub>s [] : t \<rightarrow> t'"
-inductive_cases [elim]: "\<Delta>,\<Gamma> \<turnstile>\<^sub>s f # s : t \<rightarrow> t'"
+inductive_cases [elim]: "\<Delta>,\<Gamma> \<turnstile>\<^sub>e\<^sub>c [] : t \<rightarrow> t'"
+inductive_cases [elim]: "\<Delta>,\<Gamma> \<turnstile>\<^sub>e\<^sub>c f # s : t \<rightarrow> t'"
 
 fun unfold :: "expr \<Rightarrow> frame list \<times> expr" 
 and unfold_f :: "expr list \<Rightarrow> expr list \<times> expr list \<times> frame list \<times> expr" where
@@ -68,33 +68,30 @@ and unfold_f :: "expr list \<Rightarrow> expr list \<times> expr list \<times> f
     then cons_fst e (unfold_f fs)
     else ([], fs, unfold e))"
 
-fun fold' :: "frame \<Rightarrow> expr \<Rightarrow> expr" where
-  "fold' f e = f e"
-
 fun fold :: "frame list \<Rightarrow> expr \<Rightarrow> expr" where
   "fold [] e = e"
-| "fold (f # s) e = fold' f (fold s e)"
+| "fold (f # s) e = f (fold s e)"
 
 lemma [simp]: "unfold e = (s, e') \<Longrightarrow> fold s e' = e"
   and [simp]: "unfold_f fs = (vs, nvs, s, e') \<Longrightarrow> \<not> is_value_f fs \<Longrightarrow> vs @ [fold s e'] @ nvs = fs"
   by (induction e and fs arbitrary: s e' and vs nvs s e' rule: unfold_unfold_f.induct) 
      (auto split: if_splits prod.splits)
 
-lemma [simp]: "\<Delta>,\<Gamma> \<turnstile> f : t\<^sub>1 \<rightarrow> t\<^sub>2 \<Longrightarrow> \<Delta>,\<Gamma> \<turnstile> e : t\<^sub>1 \<Longrightarrow> \<Delta>,\<Gamma> \<turnstile> fold' f e : t\<^sub>2"
+lemma [simp]: "\<Delta>,\<Gamma> \<turnstile> f : t\<^sub>1 \<rightarrow> t\<^sub>2 \<Longrightarrow> \<Delta>,\<Gamma> \<turnstile> e : t\<^sub>1 \<Longrightarrow> \<Delta>,\<Gamma> \<turnstile> f e : t\<^sub>2"
   by (induction \<Gamma> f t\<^sub>1 t\<^sub>2 rule: typecheck_frame.induct) simp_all
 
-lemma [simp]: "\<Delta>,\<Gamma> \<turnstile>\<^sub>s s : t' \<rightarrow> t \<Longrightarrow> \<Delta>,\<Gamma> \<turnstile> e : t' \<Longrightarrow> \<Delta>,\<Gamma> \<turnstile> fold s e : t"
-  by (induction \<Gamma> s t' t rule: typecheck_stack.induct) auto
+lemma [simp]: "\<Delta>,\<Gamma> \<turnstile>\<^sub>e\<^sub>c s : t' \<rightarrow> t \<Longrightarrow> \<Delta>,\<Gamma> \<turnstile> e : t' \<Longrightarrow> \<Delta>,\<Gamma> \<turnstile> fold s e : t"
+  by (induction \<Gamma> s t' t rule: typecheck_context.induct) auto
 
-lemma [simp]: "\<Delta>,\<Gamma> \<turnstile> e : t \<Longrightarrow> unfold e = (s, e') \<Longrightarrow> \<exists>t'. (\<Delta>,\<Gamma> \<turnstile>\<^sub>s s : t' \<rightarrow> t) \<and> (\<Delta>,\<Gamma> \<turnstile> e' : t')"
+lemma [simp]: "\<Delta>,\<Gamma> \<turnstile> e : t \<Longrightarrow> unfold e = (s, e') \<Longrightarrow> \<exists>t'. (\<Delta>,\<Gamma> \<turnstile>\<^sub>e\<^sub>c s : t' \<rightarrow> t) \<and> (\<Delta>,\<Gamma> \<turnstile> e' : t')"
   and [simp]: "\<Delta>,\<Gamma> \<turnstile>\<^sub>f fs : ts \<Longrightarrow> \<not> is_value_f fs \<Longrightarrow> unfold_f fs = (vs, nvs, s, e') \<Longrightarrow> 
-    \<exists>t t' vts nvts. ts = vts @ [t] @ nvts \<and> (\<Delta>,\<Gamma> \<turnstile>\<^sub>s s : t' \<rightarrow> t) \<and> (\<Delta>,\<Gamma> \<turnstile> e' : t') \<and> 
+    \<exists>t t' vts nvts. ts = vts @ [t] @ nvts \<and> (\<Delta>,\<Gamma> \<turnstile>\<^sub>e\<^sub>c s : t' \<rightarrow> t) \<and> (\<Delta>,\<Gamma> \<turnstile> e' : t') \<and> 
       (\<Delta>,\<Gamma> \<turnstile>\<^sub>f vs : vts) \<and> (\<Delta>,\<Gamma> \<turnstile>\<^sub>f nvs : nvts)"
   and [simp]: "\<Delta>,\<Gamma> \<turnstile>\<^sub>c cs : ts \<rightarrow> t \<Longrightarrow> True"
   proof (induction \<Delta> \<Gamma> e t and \<Delta> \<Gamma> fs ts arbitrary: s and vs nvs s 
          rule: typecheck_typecheck_fs_typecheck_cs.inducts)
   case (tc_var x \<Gamma> t)
-    thus ?case by simp (metis tcs_nil typecheck_typecheck_fs_typecheck_cs.tc_var)
+    thus ?case by simp (metis tcec_nil typecheck_typecheck_fs_typecheck_cs.tc_var)
   next case (tc_app \<Delta> \<Gamma> e\<^sub>1 t\<^sub>1 t\<^sub>2 e\<^sub>2)
     thus ?case 
       proof (cases "is_value e\<^sub>1")
@@ -103,98 +100,98 @@ lemma [simp]: "\<Delta>,\<Gamma> \<turnstile> e : t \<Longrightarrow> unfold e =
           proof (cases "is_value e\<^sub>2")
           case True
             with tc_app T show ?thesis 
-              by simp (metis tcs_nil typecheck_typecheck_fs_typecheck_cs.tc_app)
+              by simp (metis tcec_nil typecheck_typecheck_fs_typecheck_cs.tc_app)
           next case False
             with tc_app True obtain s\<^sub>2 where "unfold e\<^sub>2 = (s\<^sub>2, e') \<and> s = App e\<^sub>1 # s\<^sub>2" by fastforce
-            moreover with tc_app obtain t' where "(\<Delta>,\<Gamma> \<turnstile>\<^sub>s s\<^sub>2 : t' \<rightarrow> t\<^sub>1) \<and> \<Delta>,\<Gamma> \<turnstile> e' : t'" 
+            moreover with tc_app obtain t' where "(\<Delta>,\<Gamma> \<turnstile>\<^sub>e\<^sub>c s\<^sub>2 : t' \<rightarrow> t\<^sub>1) \<and> \<Delta>,\<Gamma> \<turnstile> e' : t'" 
               by fastforce
-            moreover with tc_app have "\<Delta>,\<Gamma> \<turnstile>\<^sub>s App e\<^sub>1 # s\<^sub>2 : t' \<rightarrow> t\<^sub>2" by fastforce
+            moreover with tc_app have "\<Delta>,\<Gamma> \<turnstile>\<^sub>e\<^sub>c App e\<^sub>1 # s\<^sub>2 : t' \<rightarrow> t\<^sub>2" by fastforce
             ultimately show ?thesis by fastforce
           qed
       next case False
         with tc_app obtain s\<^sub>1 where "unfold e\<^sub>1 = (s\<^sub>1, e') \<and> s = (\<lambda>e. App e e\<^sub>2) # s\<^sub>1" by fastforce
-        moreover with tc_app obtain t' where "(\<Delta>,\<Gamma> \<turnstile>\<^sub>s s\<^sub>1 : t' \<rightarrow> Arrow t\<^sub>1 t\<^sub>2) \<and> \<Delta>,\<Gamma> \<turnstile> e' : t'" 
+        moreover with tc_app obtain t' where "(\<Delta>,\<Gamma> \<turnstile>\<^sub>e\<^sub>c s\<^sub>1 : t' \<rightarrow> Arrow t\<^sub>1 t\<^sub>2) \<and> \<Delta>,\<Gamma> \<turnstile> e' : t'" 
           by fastforce
-        moreover with tc_app have "\<Delta>,\<Gamma> \<turnstile>\<^sub>s (\<lambda>e. App e e\<^sub>2) # s\<^sub>1 : t' \<rightarrow> t\<^sub>2" by fastforce
+        moreover with tc_app have "\<Delta>,\<Gamma> \<turnstile>\<^sub>e\<^sub>c (\<lambda>e. App e e\<^sub>2) # s\<^sub>1 : t' \<rightarrow> t\<^sub>2" by fastforce
         ultimately show ?thesis by fastforce
       qed
   next case (tc_abs \<Delta> t\<^sub>1 \<Gamma> e t\<^sub>2)
-    thus ?case by simp (metis tcs_nil typecheck_typecheck_fs_typecheck_cs.tc_abs)
+    thus ?case by simp (metis tcec_nil typecheck_typecheck_fs_typecheck_cs.tc_abs)
   next case (tc_let \<Delta> \<Gamma> e\<^sub>1 t\<^sub>1 e\<^sub>2 t\<^sub>2)
     thus ?case
       proof (cases "is_value e\<^sub>1")
       case True
-        with tc_let show ?thesis by simp (metis tcs_nil typecheck_typecheck_fs_typecheck_cs.tc_let)
+        with tc_let show ?thesis by simp (metis tcec_nil typecheck_typecheck_fs_typecheck_cs.tc_let)
       next case False
         with tc_let obtain s' where S: "unfold e\<^sub>1 = (s', e') \<and> s = (\<lambda>e. Let e e\<^sub>2) # s'"
           by (auto split: prod.splits)
-        with tc_let obtain t' where "(\<Delta>,\<Gamma> \<turnstile>\<^sub>s s' : t' \<rightarrow> t\<^sub>1) \<and> (\<Delta>,\<Gamma> \<turnstile> e' : t')" by fastforce
-        moreover with tc_let S have X: "\<Delta>,\<Gamma> \<turnstile>\<^sub>s s : t' \<rightarrow> t\<^sub>2" by fastforce
+        with tc_let obtain t' where "(\<Delta>,\<Gamma> \<turnstile>\<^sub>e\<^sub>c s' : t' \<rightarrow> t\<^sub>1) \<and> (\<Delta>,\<Gamma> \<turnstile> e' : t')" by fastforce
+        moreover with tc_let S have X: "\<Delta>,\<Gamma> \<turnstile>\<^sub>e\<^sub>c s : t' \<rightarrow> t\<^sub>2" by fastforce
         ultimately show ?thesis by fastforce
       qed
   next case (tc_rec \<Delta> \<Gamma> fs ts)
     thus ?case 
       proof (cases "is_value_f fs")
       case True
-        with tc_rec show ?thesis by simp (metis tcs_nil typecheck_typecheck_fs_typecheck_cs.tc_rec)
+        with tc_rec show ?thesis by simp (metis tcec_nil typecheck_typecheck_fs_typecheck_cs.tc_rec)
       next case False
         then obtain vs nvs ss ee' where F: "unfold_f fs = (vs, nvs, ss, ee')" 
           by (cases "unfold_f fs") simp_all
         with tc_rec False obtain t t' vts nvts where T: "ts = vts @ [t] @ nvts \<and> 
-          (\<Delta>,\<Gamma> \<turnstile>\<^sub>s ss : t' \<rightarrow> t) \<and> (\<Delta>,\<Gamma> \<turnstile> e' : t') \<and> (\<Delta>,\<Gamma> \<turnstile>\<^sub>f vs : vts) \<and> \<Delta>,\<Gamma> \<turnstile>\<^sub>f nvs : nvts" 
+          (\<Delta>,\<Gamma> \<turnstile>\<^sub>e\<^sub>c ss : t' \<rightarrow> t) \<and> (\<Delta>,\<Gamma> \<turnstile> e' : t') \<and> (\<Delta>,\<Gamma> \<turnstile>\<^sub>f vs : vts) \<and> \<Delta>,\<Gamma> \<turnstile>\<^sub>f nvs : nvts" 
             by fastforce
-        hence "\<Delta>,\<Gamma> \<turnstile>\<^sub>s (\<lambda>e. Rec (vs @ [e] @ nvs)) # ss : t' \<rightarrow> Record ts" by fastforce
+        hence "\<Delta>,\<Gamma> \<turnstile>\<^sub>e\<^sub>c (\<lambda>e. Rec (vs @ [e] @ nvs)) # ss : t' \<rightarrow> Record ts" by fastforce
         with tc_rec False F T show ?thesis by fastforce
       qed
   next case (tc_proj \<Delta> \<Gamma> e ts l t)
     thus ?case
       proof (cases "is_value e")
       case True
-        with tc_proj show ?thesis by simp (metis tcs_nil typecheck_typecheck_fs_typecheck_cs.tc_proj)
+        with tc_proj show ?thesis by simp (metis tcec_nil typecheck_typecheck_fs_typecheck_cs.tc_proj)
       next case False
         with tc_proj obtain ss where "unfold e = (ss, e') \<and> s = (\<lambda>e. Proj e l) # ss" 
           by (auto split: prod.splits)
-        moreover with tc_proj obtain t' where "(\<Delta>,\<Gamma> \<turnstile>\<^sub>s ss : t' \<rightarrow> Record ts) \<and> (\<Delta>,\<Gamma> \<turnstile> e' : t')" 
+        moreover with tc_proj obtain t' where "(\<Delta>,\<Gamma> \<turnstile>\<^sub>e\<^sub>c ss : t' \<rightarrow> Record ts) \<and> (\<Delta>,\<Gamma> \<turnstile> e' : t')" 
           by fastforce
-        moreover with tc_proj have "\<Delta>,\<Gamma> \<turnstile>\<^sub>s (\<lambda>e. Proj e l) # ss : t' \<rightarrow> t" by fastforce
+        moreover with tc_proj have "\<Delta>,\<Gamma> \<turnstile>\<^sub>e\<^sub>c (\<lambda>e. Proj e l) # ss : t' \<rightarrow> t" by fastforce
         ultimately show ?thesis by fastforce
       qed
   next case (tc_inj \<Delta> \<Gamma> e t l ts)
     thus ?case
       proof (cases "is_value e")
       case True
-        with tc_inj show ?thesis by simp (metis tcs_nil typecheck_typecheck_fs_typecheck_cs.tc_inj)
+        with tc_inj show ?thesis by simp (metis tcec_nil typecheck_typecheck_fs_typecheck_cs.tc_inj)
       next case False
         with tc_inj obtain s' where S: "unfold e = (s', e') \<and> s = Inj l ts # s'" 
           by (auto split: prod.splits)
-        with tc_inj obtain t' where "(\<Delta>,\<Gamma> \<turnstile>\<^sub>s s' : t' \<rightarrow> t) \<and> (\<Delta>,\<Gamma> \<turnstile> e' : t')" by fastforce
-        moreover with tc_inj S have "\<Delta>,\<Gamma> \<turnstile>\<^sub>s s : t' \<rightarrow> Variant ts" by fastforce
+        with tc_inj obtain t' where "(\<Delta>,\<Gamma> \<turnstile>\<^sub>e\<^sub>c s' : t' \<rightarrow> t) \<and> (\<Delta>,\<Gamma> \<turnstile> e' : t')" by fastforce
+        moreover with tc_inj S have "\<Delta>,\<Gamma> \<turnstile>\<^sub>e\<^sub>c s : t' \<rightarrow> Variant ts" by fastforce
         ultimately show ?thesis by fastforce
       qed
   next case (tc_case \<Delta> \<Gamma> e ts cs t)
     thus ?case
       proof (cases "is_value e")
       case True
-        with tc_case show ?thesis by simp (metis tcs_nil typecheck_typecheck_fs_typecheck_cs.tc_case)
+        with tc_case show ?thesis by simp (metis tcec_nil typecheck_typecheck_fs_typecheck_cs.tc_case)
       next case False
         with tc_case obtain s' where S: "unfold e = (s', e') \<and> s = (\<lambda>e. Case e cs) # s'" 
           by (auto split: prod.splits)
-        with tc_case obtain t' where T: "(\<Delta>,\<Gamma> \<turnstile>\<^sub>s s' : t' \<rightarrow> Variant ts) \<and> (\<Delta>,\<Gamma> \<turnstile> e' : t')" 
+        with tc_case obtain t' where T: "(\<Delta>,\<Gamma> \<turnstile>\<^sub>e\<^sub>c s' : t' \<rightarrow> Variant ts) \<and> (\<Delta>,\<Gamma> \<turnstile> e' : t')" 
           by fastforce
-        with tc_case S have "\<Delta>,\<Gamma> \<turnstile>\<^sub>s s : t' \<rightarrow> t" by fastforce
+        with tc_case S have "\<Delta>,\<Gamma> \<turnstile>\<^sub>e\<^sub>c s : t' \<rightarrow> t" by fastforce
         with T show ?thesis by fastforce
       qed
   next case (tc_fold \<Delta> \<Gamma> e t)
     thus ?case
       proof (cases "is_value e")
       case True
-        with tc_fold show ?thesis by simp (metis tcs_nil typecheck_typecheck_fs_typecheck_cs.tc_fold)
+        with tc_fold show ?thesis by simp (metis tcec_nil typecheck_typecheck_fs_typecheck_cs.tc_fold)
       next case False
         with tc_fold obtain s' where S: "unfold e = (s', e') \<and> s = Fold t # s'"
           by (auto split: prod.splits)
-        with tc_fold obtain t' where T: "(\<Delta>,\<Gamma> \<turnstile>\<^sub>s s' : t' \<rightarrow> subst\<^sub>t\<^sub>t 0 (Inductive t) t) \<and> 
+        with tc_fold obtain t' where T: "(\<Delta>,\<Gamma> \<turnstile>\<^sub>e\<^sub>c s' : t' \<rightarrow> subst\<^sub>t\<^sub>t 0 (Inductive t) t) \<and> 
           (\<Delta>,\<Gamma> \<turnstile> e' : t')" by fastforce
-        with tc_fold S have "\<Delta>,\<Gamma> \<turnstile>\<^sub>s s : t' \<rightarrow> Inductive t" by fastforce
+        with tc_fold S have "\<Delta>,\<Gamma> \<turnstile>\<^sub>e\<^sub>c s : t' \<rightarrow> Inductive t" by fastforce
         with T show ?thesis by fastforce
       qed
   next case (tc_unfold \<Delta> \<Gamma> e t)
@@ -202,33 +199,33 @@ lemma [simp]: "\<Delta>,\<Gamma> \<turnstile> e : t \<Longrightarrow> unfold e =
       proof (cases "is_value e")
       case True
         with tc_unfold show ?thesis 
-          by simp (metis tcs_nil typecheck_typecheck_fs_typecheck_cs.tc_unfold)
+          by simp (metis tcec_nil typecheck_typecheck_fs_typecheck_cs.tc_unfold)
       next case False
         with tc_unfold obtain s' where S: "unfold e = (s', e') \<and> s = Unfold t # s'"
           by (auto split: prod.splits)
-        with tc_unfold obtain t' where T: "(\<Delta>,\<Gamma> \<turnstile>\<^sub>s s' : t' \<rightarrow> Inductive t) \<and> 
+        with tc_unfold obtain t' where T: "(\<Delta>,\<Gamma> \<turnstile>\<^sub>e\<^sub>c s' : t' \<rightarrow> Inductive t) \<and> 
           (\<Delta>,\<Gamma> \<turnstile> e' : t')" by fastforce
-        with tc_unfold S have "\<Delta>,\<Gamma> \<turnstile>\<^sub>s s : t' \<rightarrow> subst\<^sub>t\<^sub>t 0 (Inductive t) t" by fastforce
+        with tc_unfold S have "\<Delta>,\<Gamma> \<turnstile>\<^sub>e\<^sub>c s : t' \<rightarrow> subst\<^sub>t\<^sub>t 0 (Inductive t) t" by fastforce
         with T show ?thesis by fastforce
       qed
   next case (tc_tyabs \<Delta> \<Gamma> e t)
-    thus ?case by simp (metis tcs_nil typecheck_typecheck_fs_typecheck_cs.tc_tyabs)
+    thus ?case by simp (metis tcec_nil typecheck_typecheck_fs_typecheck_cs.tc_tyabs)
   next case (tc_tyapp \<Delta> \<Gamma> e t t')
     thus ?case
       proof (cases "is_value e")
       case True
         with tc_tyapp show ?thesis 
-          by simp (metis tcs_nil typecheck_typecheck_fs_typecheck_cs.tc_tyapp)
+          by simp (metis tcec_nil typecheck_typecheck_fs_typecheck_cs.tc_tyapp)
       next case False
         with tc_tyapp obtain s' where S: "unfold e = (s', e') \<and> s = (\<lambda>e. TyApp e t') # s'" 
           by (auto split: prod.splits)
-        with tc_tyapp obtain tt where T: "(\<Delta>,\<Gamma> \<turnstile>\<^sub>s s' : tt \<rightarrow> Forall t) \<and> (\<Delta>,\<Gamma> \<turnstile> e' : tt)" 
+        with tc_tyapp obtain tt where T: "(\<Delta>,\<Gamma> \<turnstile>\<^sub>e\<^sub>c s' : tt \<rightarrow> Forall t) \<and> (\<Delta>,\<Gamma> \<turnstile> e' : tt)" 
           by fastforce
-        with tc_tyapp have "\<Delta>,\<Gamma> \<turnstile>\<^sub>s (\<lambda>e. TyApp e t') # s' : tt \<rightarrow> subst\<^sub>t\<^sub>t 0 t' t" by fastforce
+        with tc_tyapp have "\<Delta>,\<Gamma> \<turnstile>\<^sub>e\<^sub>c (\<lambda>e. TyApp e t') # s' : tt \<rightarrow> subst\<^sub>t\<^sub>t 0 t' t" by fastforce
         with S T show ?thesis by fastforce
       qed
   next case (tc_tylet \<Delta> \<Gamma> t' e t)
-    thus ?case by simp (metis tcs_nil typecheck_typecheck_fs_typecheck_cs.tc_tylet)
+    thus ?case by simp (metis tcec_nil typecheck_typecheck_fs_typecheck_cs.tc_tylet)
   next case (tcf_cons \<Delta> \<Gamma> e tt fs ts)
     thus ?case
       proof (cases "is_value e")
@@ -236,13 +233,13 @@ lemma [simp]: "\<Delta>,\<Gamma> \<turnstile> e : t \<Longrightarrow> unfold e =
         with tcf_cons obtain vs' where V: "unfold_f fs = (vs', nvs, s, e') \<and> vs = e # vs'" 
           by (cases "unfold_f fs") fastforce+
         moreover with tcf_cons True obtain t t' vts nvts where T: "ts = vts @ [t] @ nvts \<and> 
-          (\<Delta>,\<Gamma> \<turnstile>\<^sub>s s : t' \<rightarrow> t) \<and> (\<Delta>,\<Gamma> \<turnstile> e' : t') \<and> (\<Delta>,\<Gamma> \<turnstile>\<^sub>f vs' : vts) \<and> \<Delta>,\<Gamma> \<turnstile>\<^sub>f nvs : nvts" 
+          (\<Delta>,\<Gamma> \<turnstile>\<^sub>e\<^sub>c s : t' \<rightarrow> t) \<and> (\<Delta>,\<Gamma> \<turnstile> e' : t') \<and> (\<Delta>,\<Gamma> \<turnstile>\<^sub>f vs' : vts) \<and> \<Delta>,\<Gamma> \<turnstile>\<^sub>f nvs : nvts" 
             by fastforce
         moreover hence "tt # ts = (tt # vts) @ [t] @ nvts" by simp
         moreover from tcf_cons V T have "\<Delta>,\<Gamma> \<turnstile>\<^sub>f vs : tt # vts" by simp
         ultimately show ?thesis by blast
       next case False
-        with tcf_cons obtain t' where "(\<Delta>,\<Gamma> \<turnstile>\<^sub>s s : t' \<rightarrow> tt) \<and> \<Delta>,\<Gamma> \<turnstile> e' : t'" by fastforce
+        with tcf_cons obtain t' where "(\<Delta>,\<Gamma> \<turnstile>\<^sub>e\<^sub>c s : t' \<rightarrow> tt) \<and> \<Delta>,\<Gamma> \<turnstile> e' : t'" by fastforce
         moreover from tcf_cons False have "\<Delta>,\<Gamma> \<turnstile>\<^sub>f vs : []" by simp
         moreover from tcf_cons False have "\<Delta>,\<Gamma> \<turnstile>\<^sub>f nvs : ts" by simp
         ultimately show ?thesis by fastforce
